concur/HCompBack.v
@@ -1,0 +1,367 @@
+Require Import Coqlib.
+Require Import List.
+Require Import Events.
+Require Import Memory.
+Require Import Globalenvs.
+Require Import LanguageInterface.
+Require Import Smallstep CallconvBig.
+Require Import Linking.
+Require Import Classical.
+Require Import HCompBig.
+
+
+Section BSIM.
+  Context {li1 li2} (cc: callconv li1 li2).
+
+  Notation I := bool.
+  Context (L1 : I -> Smallstep.semantics li1 li1).
+  Context (L2 : I -> Smallstep.semantics li2 li2).
+  Context (HL : forall i, bsim_components cc cc (L1 i) (L2 i)).
+  Context (se1 se2: Genv.symtbl) (w : ccworld cc).
+  Context (Hse: match_senv cc w se1 se2).
+  Context (Hse1: forall i, Genv.valid_for (skel (L1 i)) se1).
+  Notation index := {i & bsim_index (HL i)}.
+
+  Inductive match_topframes_back wk : GS.gworld cc -> index -> bool -> frame L1 -> frame L2 -> Prop :=
+    match_topframes_intro gw i s1 s2 idx:
+      match_senv cc wk se1 se2 ->
+      Genv.valid_for (skel (L1 i)) se1 ->
+      bsim_match_states (HL i) se1 se2 wk idx s1 s2 ->
+      match_topframes_back wk gw
+        (existT _ i idx) i
+        (st L1 i s1)
+        (st L2 i s2).
+
+  Inductive match_contframes wk wk': bool -> frame L1 -> frame L2 -> Prop :=
+    match_contframes_intro i s1 s2:
+      match_senv cc wk' se1 se2 ->
+      (forall r1 r2, match_reply cc wk r1 r2 ->
+     bsim_match_cont (rex (bsim_match_states (HL i) se1 se2 wk'))
+       (Smallstep.after_external (L1 i se1) s1 r1)
+       (Smallstep.after_external (L2 i se2) s2 r2)) ->
+      match_contframes wk wk' i
+        (st L1 i s1)
+        (st L2 i s2).
+
+  Inductive match_states: index -> list (frame L1) -> list (frame L2) -> Prop :=
+    | match_states_cons wk idx f1 f2 k1 k2 i j:
+        match_topframes wk idx i f1 f2 ->
+        match_cont wk j k1 k2 ->
+        i <> j ->
+        match_states idx (f1 :: k1) (f2 :: k2)
+  with match_cont: ccworld cc -> bool -> _ -> _ -> Prop :=
+    | match_cont_cons wk wk' f1 f2 k1 k2 i j:
+        match_contframes wk wk' i f1 f2 ->
+        match_cont wk' j k1 k2 ->
+        i <> j ->
+        match_cont wk i (f1 :: k1) (f2 :: k2)
+    | match_cont_nil i:
+        match_cont w i nil nil.
+
+  Inductive order: index -> index -> Prop :=
+    order_intro i x y: bsim_order (HL i) x y -> order (existT _ i x) (existT _ i y).
+
+  (** semantics bsim_properties *)
+
+  Lemma safe_internal : forall (i:I) s1 k1,
+      safe L1 se1 (st L1 i s1 :: k1) -> Smallstep.safe (L1 i se1) s1.
+  Proof.
+    intros.
+    red. intros.
+    red in H. exploit H. eapply star_internal; eauto.
+    intros [[r A] | [[q B] | [t [s2' C]]]].
+    - inv A. subst_dep. left. eauto.
+    - inv B. subst_dep. right. left. eauto.
+    - inv C. subst_dep. right. right. eauto.
+      subst_dep. right. left. eauto.
+      subst_dep. left. eauto.
+  Qed.
+
+  Hypothesis determinate_L1: forall i, determinate_big (L1 i).
+  
+  Lemma step_simulation:
+    forall idx s1 s2 t s2', match_states idx s1 s2 -> step L2 se2 s2 t s2' -> safe L1 se1 s1 ->
+    exists idx' s1',
+      (plus (fun _ => step L1 se1) tt s1 t s1' \/
+       star (fun _ => step L1 se1) tt s1 t s1' /\ order idx' idx) /\
+      match_states idx' s1' s2'.
+  Proof.
+    intros idx s1 s2 t s2' Hs Hs1' Hsafe.
+    destruct Hs1'; inv Hs.
+    - (* internal step *)
+      remember (st L2 i s) as f2.
+      inv H2. inv H9. subst_dep.
+      (* inv H4; subst_dep. clear idx0. *)
+      edestruct @bsim_simulation as (idx' & s2' & Hs2' & Hs'); eauto using bsim_lts.
+      eapply safe_internal; eauto.
+      eexists (existT _ i idx'), _. split.
+      * destruct Hs2'; [left | right]; intuition eauto using star_internal, plus_internal.
+        constructor. auto.
+      * econstructor; eauto. econstructor; eauto.
+    - (* cross-component call *)
+      remember (st L2 i s) as f2. inv H5. inv H12. subst_dep.
+      edestruct @bsim_match_external as (wx & s1' & qx1 & Hsteps1 & Hqx1 & Hqx & Hsex & Hrx); eauto using bsim_lts.
+      eapply safe_internal; eauto.
+      pose proof (determinate_L1 i se1) as DETERMi1.
+      exploit Hsafe; eauto. eapply star_internal; eauto. rename q into q2.
+      intros [[r1' Final1] | [[q1 Ext1] | [t [s2' Step1]]]].
+      + inv Final1. subst_dep. exfalso. eapply @sd_big_final_noext; eauto.
+      + inv Ext1. subst_dep. exfalso. exploit @sd_big_at_external_determ. eauto.
+        apply Hqx1. apply H12. intro. subst qx1.
+        pose proof (bsim_lts (HL j) _ _ Hsex (Hse1 j)).
+        erewrite bsim_match_valid_query in H0; eauto. congruence.
+      + inv Step1; subst_dep.
+        -- exfalso. eapply @sd_big_at_external_nostep; eauto.
+        -- exploit @sd_big_at_external_determ. eauto.
+           apply Hqx1. apply H11. intro. subst qx1.
+           pose proof (bsim_lts (HL j1) _ _ Hsex (Hse1 j1)).
+           exploit @bsim_match_initial_states; eauto.
+           intros HrexI. inv HrexI.
+           assert (j0 = j1).
+           { destruct j0; destruct j1; destruct i; congruence. }
+           subst j1. assert (j0 = j).
+           { destruct j0; destruct j; destruct i; congruence. }
+           subst j0.
+           exploit bsim_match_cont_match; eauto.
+           intros [s1j' [HIj1 [idx' Hmsj]]].
+           eexists. eexists. split.
+           left. eapply plus_right. eapply star_internal; eauto.
+           eapply step_push; eauto. reflexivity.
+           econstructor.
+           econstructor; eauto. econstructor; eauto. econstructor; eauto. eauto.
+        -- exfalso. eapply @sd_big_final_noext; eauto.
+    - (* cross-component return *)
+      remember (st L2 i s) as f2.
+      inv H4. inv H11. subst_dep. clear idx0.
+      pose proof (bsim_lts (HL i) _ _ H2 H3).
+      apply safe_internal in Hsafe as Hsafei.
+      edestruct @bsim_match_final_states as (s2' & r2 & Hstar2 & Hr2 & Hr); eauto.
+      remember (st L2 j sk :: k) as k2.
+      inv H7; try congruence. inv H14.
+      remember (st L2 j sk) as f2. inv H6. inv H14.
+      subst_dep. specialize (H11 _ _ Hr).
+      inv H11.
+      pose proof (determinate_L1 i se1) as DETERMi1.
+      exploit Hsafe; eauto. eapply star_internal; eauto.
+      intros [[r1' Final1] | [[q1 Ext1] | [t [s2'' Step1]]]].
+      + inv Final1.
+      + inv Ext1. subst_dep. exfalso. exploit @sd_big_final_noext; eauto.
+      + inv Step1; subst_dep.
+        -- exfalso. exploit @sd_big_final_nostep; eauto.
+        -- exfalso. exploit @sd_big_final_noext; eauto.
+        -- exploit @sd_big_final_determ. eauto. apply Hr2. apply H17. intro.
+           subst r0.
+           assert (j1 = i). {destruct j1; destruct i; destruct j; congruence. }
+           subst j1.
+           exploit bsim_match_cont_match; eauto.
+           intros (s1j' & HY1j & idxj & Hmsj).
+           eexists. eexists. split.
+           left. eapply plus_right. eapply star_internal; eauto.
+           eapply step_pop; eauto. reflexivity.
+           econstructor; eauto. econstructor; eauto.
+  Qed.
+  (* bsim_properties *)
+
+  Hypothesis valid_query_excl:
+    forall i j se q,
+      Smallstep.valid_query (L1 i se) q = true ->
+      Smallstep.valid_query (L1 j se) q = true ->
+      i = j.
+  
+  Lemma match_query_excl : forall q1 q2 i j,
+      match_query cc w q1 q2 ->
+      Smallstep.valid_query (L1 i se1) q1 = true ->
+      Smallstep.valid_query (L2 j se2) q2 = true ->
+      i = j.
+  Proof.
+    intros.  pose proof (bsim_lts (HL j) _ _ Hse (Hse1 j)).
+    erewrite bsim_match_valid_query in H1; eauto.
+  Qed.
+    
+  Lemma initial_states_simulation:
+    forall q1 q2, match_query cc w q1 q2 ->
+                bsim_match_cont (rex match_states) (initial_state L1 se1 q1) (initial_state L2 se2 q2).
+  Proof.
+    intros q1 q2 Hq. constructor.
+    - intros _ [i s1' Hq1 Hs1].
+      pose proof (bsim_lts (HL i) _ _ Hse (Hse1 i)). inv H.
+      exploit bsim_match_initial_states; eauto. intro.
+      inv H. exploit bsim_match_cont_exist; eauto. intros (s2 & Hi2).
+      eexists. econstructor; eauto.
+    - intros sl1 sl2 [i s1' Hq1 Hs1] [j s2' Hq2 Hs2].
+      exploit match_query_excl; eauto. intro. subst j.
+      pose proof (bsim_lts (HL i) _ _ Hse (Hse1 i)). inv H.
+      exploit bsim_match_initial_states; eauto. intro.
+      inv H. exploit bsim_match_cont_match; eauto. intros (s1'' & Hi1' & Hrex).
+      eexists. split. econstructor; eauto. inv Hrex.
+      eexists. econstructor; eauto. econstructor; eauto.
+      instantiate (1:= negb i).
+      constructor. destruct i; simpl; congruence.
+  Qed.
+
+  Lemma final_states_simulation:
+    forall idx s1 s2 r2,
+      match_states idx s1 s2 ->
+      safe L1 se1 s1 ->
+      final_state L2 se2 s2 r2 ->
+      exists s1' r1, star (fun _ => step L1 se1) tt s1 E0 s1' /\
+        final_state L1 se1 s1' r1 /\ match_reply cc w r1 r2.
+  Proof.
+    clear. intros idx s1 s2 r2 Hs Hsafe Hr2. destruct Hr2 as [i s2 r2 Hr2].
+    inv Hs. inv H4. remember (st L2 i s2) as f2. inv H1. inv H7. subst_dep.
+    pose proof (bsim_lts (HL i) _ _ H H0).
+    edestruct @bsim_match_final_states as (s1' & r1 & Hstar & Hr1 & Hr); eauto.
+    eapply safe_internal; eauto.
+    eexists. exists r1. split. eapply star_internal; eauto.
+    split; eauto. constructor; eauto.
+  Qed.
+  
+  Lemma external_simulation:
+    forall idx s1 s2 qx2, match_states idx s1 s2 -> safe L1 se1 s1 -> at_external L2 se2 s2 qx2 ->
+    exists wx s1' qx1, star (fun _ => step L1 se1) tt s1 E0 s1' /\ at_external L1 se1 s1' qx1 /\ match_query cc wx qx1 qx2 /\ match_senv cc wx se1 se2 /\
+    forall rx1 rx2, match_reply cc wx rx1 rx2 -> bsim_match_cont (rex match_states) (after_external L1 se1 s1' rx1)
+                                             (after_external L2 se2 s2 rx2).
+  Proof.
+    clear - HL Hse1.
+    intros idx s1 s2 q2 Hs Hsafe Hq2. destruct Hq2 as [i s2 qx2 k2 Hqx2 Hvld].
+    inv Hs. remember (st L2 i s2) as f2. inv H1. inv H8. subst_dep.
+    pose proof (bsim_lts (HL i) _ _ H H0) as Hi.
+    edestruct @bsim_match_external as (wx & s1' & qx1 & Hstar & Hqx1 & Hqx & Hsex & Hr); eauto.
+    eapply safe_internal; eauto.
+    exists wx. eexists. exists qx1. intuition idtac.
+    + eapply star_internal; eauto.
+    + constructor. eauto.
+      intros j0. pose proof (bsim_lts (HL j0) _ _ Hsex (Hse1 j0)).
+      erewrite <- bsim_match_valid_query; eauto.
+    + exploit Hr; eauto. intros.  inv H3.
+      constructor.
+      -- intros s1'' Hy1. inv Hy1. subst_dep.
+         exploit bsim_match_cont_exist; eauto.
+         intros (s2'' & Hy2). eexists. econstructor; eauto.
+      -- intros s1'' s2'' Hy1 Hy2. inv Hy1. inv Hy2. subst_dep.
+         exploit bsim_match_cont_match; eauto.
+         intros (s1'''  & Hy1' & Hrex).
+         eexists. split. econstructor; eauto. inv Hrex. eexists.
+         econstructor; eauto. econstructor; eauto.
+  Qed.
+
+  Lemma progress_simulation :
+    forall idx s1 s2, match_states idx s1 s2 -> safe L1 se1 s1 ->
+                  (exists r, final_state L2 se2 s2 r) \/
+                  (exists q, at_external L2 se2 s2 q) \/
+                    (exists t s2', step L2 se2 s2 t s2').
+  Proof.
+    intros. inv H. inv H1. subst_dep.
+    assert (SAFE_L1i: Smallstep.safe (L1 i se1) s1).
+    eapply safe_internal; eauto.
+    pose proof (bsim_lts (HL i) _ _ H (Hse1 i)).
+    exploit @bsim_progress; eauto.
+    pose proof (determinate_L1 i se1).
+    intros [[r Final2i] | [[q Ext2i] | [t [s2' Step2i]]]].
+    - (** the top target semantics L2 i enters a final state *)
+      exploit @bsim_match_final_states; eauto.
+      intros (s1' & r1 & Star1 & Final1i & MR).
+      (** the top source semantics L1 i also finals by bsim*)
+      exploit H0. eapply star_internal; eauto.
+      intros [[r1' Final1] | [[q Ext1] | [t [s2' Step1]]]].
+      + (** the source semantics finals, i.e. with empty state stack *)
+        inv Final1. subst_dep. left. inv H2. econstructor; eauto.
+        econstructor; eauto.
+      + inv Ext1. subst_dep.
+        exfalso.
+        exploit @sd_big_final_noext; eauto.
+      + inv Step1. subst_dep.
+        -- exfalso. exploit @sd_big_final_nostep; eauto.
+        -- subst_dep. exfalso. exploit @sd_big_final_noext; eauto.
+        -- subst_dep. inv H2.
+           assert (j1 = i).
+           { destruct j; destruct j1; destruct i; congruence. }
+           subst j1.
+           assert (j0 = j).
+           { destruct j; destruct j0; destruct i; congruence. }
+           subst j0.
+           right. right.
+           exploit @sd_big_final_determ. eauto. apply Final1i. apply H10. intro. subst r0.
+           inv H9. subst_dep.
+           exploit H11. eauto. intro. inv H2.
+           exploit bsim_match_cont_exist; eauto.
+           intros [s2' AFTER2j].
+           eexists. eexists.
+           eapply step_pop; eauto.
+    - (** the top target semantics L2 i [at_external]s *)
+      exploit @bsim_match_external; eauto. rename q into q2.
+      intros (wA & s1' & q1 & HStar & X1i & MQ & MS & MR).
+      exploit H0; eauto. eapply star_internal; eauto.
+      intros [[r1' Final1] | [[q Ext1] | [t [s2' Step1]]]].
+      + (** the source semantics finals, i.e. with empty state stack *)
+        inv Final1. subst_dep. exfalso. eapply @sd_big_final_noext; eauto.
+      + inv Ext1. subst_dep. right. left.
+        exploit @sd_big_at_external_determ. eauto. apply X1i. apply H11. intro.
+        subst q. exists q2. econstructor; eauto.
+        intros j0. pose proof (bsim_lts (HL j0) _ _ MS (Hse1 j0)).
+        erewrite bsim_match_valid_query; eauto.
+      + inv Step1. subst_dep.
+        -- exfalso. exploit @sd_big_at_external_nostep; eauto.
+        -- subst_dep. right. right.
+           exploit @sd_big_at_external_determ. eauto. apply X1i. apply H10.
+           intro. subst q.
+           pose proof (bsim_lts (HL j0) _ _ MS (Hse1 j0)).
+           exploit @bsim_match_initial_states. apply H7. eauto.
+           intro Hrexj0. inv Hrexj0. exploit bsim_match_cont_exist; eauto.
+           intros [s2' I2j0]. do 2 eexists.
+           eapply step_push. eauto. 
+           erewrite bsim_match_valid_query; eauto. eauto. eauto.
+        -- subst_dep. exfalso. eapply @sd_big_final_noext; eauto.
+    - right. right. do 2 eexists. econstructor; eauto.
+  Qed.
+
+  Lemma semantics_simulation sk1 sk2:
+    bsim_properties cc cc se1 se2 w
+      (semantics L1 sk1 se1)
+      (semantics L2 sk2 se2)
+      index order match_states.
+  Proof.
+    split; cbn.
+    - intros. unfold valid_query. f_equal.
+      + eapply (bsim_lts (HL true)); eauto.
+      + eapply (bsim_lts (HL false)); eauto.
+    - eauto using initial_states_simulation.
+    - eauto using final_states_simulation.
+    - eauto using external_simulation.
+    - eauto using progress_simulation.
+    - eauto using step_simulation.
+  Qed.
+  
+End BSIM.
+
+(** * Linking operator *)
+
+Lemma compose_simulation {li1 li2} (cc: callconv li1 li2) L1a L1b L1 L2a L2b L2:
+  backward_simulation cc cc L1a L2a ->
+  backward_simulation cc cc L1b L2b ->
+  determinate_big L1a -> determinate_big L1b ->
+  (forall q se, ~ ((Smallstep.valid_query (L1a se)) q = true /\ Smallstep.valid_query (L1b se) q = true)) ->
+  compose L1a L1b = Some L1 ->
+  compose L2a L2b = Some L2 ->
+  backward_simulation cc cc L1 L2.
+Proof.
+  intros [Ha] [Hb] Hd1 Hd2 Hqex H1 H2. unfold compose in *. unfold option_map in *.
+  destruct (link (skel L1a) (skel L1b)) as [sk1|] eqn:Hsk1; try discriminate. inv H1.
+  destruct (link (skel L2a) (skel L2b)) as [sk2|] eqn:Hsk2; try discriminate. inv H2.
+  set (L1 := fun i:bool => if i then L1a else L1b).
+  set (L2 := fun i:bool => if i then L2a else L2b).
+  assert (HL: forall i, bsim_components cc cc (L1 i) (L2 i)) by (intros [|]; auto).
+  constructor.
+  eapply Backward_simulation with (order cc L1 L2 HL) (match_states cc L1 L2 HL).
+  - destruct Ha, Hb. cbn. congruence.
+  - intros se1 se2 w Hse Hse1.
+    eapply semantics_simulation; eauto.
+    + pose proof (link_linkorder _ _ _ Hsk1) as [Hsk1a Hsk1b].
+      intros [|]; cbn; eapply Genv.valid_for_linkorder; eauto.
+      (** preconditions introduced above *)
+    + intros. destruct i; eauto.
+    + intros. destruct i; destruct j; simpl in *; eauto; exfalso; eapply Hqex; eauto.        
+  - clear - HL. intros [i x].
+    induction (bsim_order_wf (HL i) x) as [x Hx IHx].
+    constructor. intros z Hxz. inv Hxz; subst_dep. eauto.
+Qed.
